README.md
@@ -1,16 +1,15 @@
-% Verifiably Lazy : A Verified Compiler for Call-By-Need.
+# Verifiably Lazy : A Verified Compiler for Call-By-Need.
 
 # Building / Proof Checking
 
 Requirements: 
-- `coqc` and `coqdep` (tested with 8.4)
+- `coqc` and `coqdep` (tested with 8.4pl6)
 - `runhaskell` and Shake
 
 To Build: `./build.hs` (requires runhaskell and Shake, the Haskell build system) 
 
 Notes: 
-We use the convention that filenames correspond to that datatype and theorems
-, supporting datatypes, transitions for those datatypes, while filenames with
-underscores, e.g.  `c1_c2.v` represents the connections between `c1` and
-`c2`. 
+We use the convention that filenames without underscores correspond to semantics
+while relations between semantics use underscores, e.g.  `c1_c2.v` contains the
+relations between `c1` and `c2`. 
 
